
\subsection*{Three Subgroups}

First here we assume $\Var(\gamma_i) = 1$ and $\Cov(\gamma_i, \gamma_j) = 0$ for $i \neq j$

let $\beta_i = (\gamma_i - \E(\gamma_i)$

\begin{align*}
	E J_i = &p_1 ( (1 - c_1 \bar{y}_1) \beta_1 - c_1 \bar{y}_2 \beta_2 - c_1 \bar{y}_3 \beta_3 )^2 \\
		  + &p_2 ( - c_2 \bar{y}_1 \beta_1 + (1 - c_2 \bar{y}_2) \beta_2  - c_2 \bar{y}_3 \beta_3 )^2 \\
		  + &p_3 ( - c_3 \bar{y}_1 \beta_1 - c_3 \bar{y}_2 \beta_2 + (1 - c_3 \bar{y}_3) \beta_3 )^2 \\
\end{align*}
 \begin{align*}
	1 - \bar{y}_1 - \bar{y}_2 = \bar{y}_3 \\
\end{align*}


Now recall that for individual $i$,
\begin{align*}
	c_i &= \frac{\bar{y}_i}{\bar{y}_1^2 + \bar{y}_2^2 + \bar{y}_3^2} \quad \text{for $i \in \{1,\ldots,3\}$} \\
		&= \frac{\bar{y}_i}{\bar{y}_1^2 + \bar{y}_2^2 + (1 - \bar{y}_1 - \bar{y}_2 )^2} \quad \text{for $i \in \{1,\ldots,2\}$} \\
\end{align*}


also we can rewrite

\begin{align*}
	E J_i &= p_1 ( \beta_1 - c_1 (\bar{y}_1 \beta_1 + \bar{y}_2 \beta_2 + \bar{y}_3 \beta_3 ))^2 \\
		  &+ p_2 ( \beta_2 - c_2 (\bar{y}_1 \beta_1 +  \bar{y}_2 \beta_2 + \bar{y}_3 \beta_3 ))^2 \\
		  &+ p_3 ( \beta_3 - c_3 (\bar{y}_1 \beta_1 +\bar{y}_2 \beta_2 + \bar{y}_3 \beta_3 ))^2 \\
		  &= p_1 ( \beta_1 - c_1 (\bar{y}_1 \beta_1 + \bar{y}_2 \beta_2 + (1 - \bar{y}_1 - \bar{y}_2) \beta_3 ))^2 \\
		  &+ p_2 ( \beta_2 - c_2 (\bar{y}_1 \beta_1 +  \bar{y}_2 \beta_2 + (1 - \bar{y}_1 - \bar{y}_2) \beta_3 ))^2 \\
		  &+ p_3 ( \beta_3 - c_3 (\bar{y}_1 \beta_1 +\bar{y}_2 \beta_2 + (1 - \bar{y}_1 - \bar{y}_2) \beta_3 ))^2 \\
\end{align*}

expanding $c_i$ 

We can describe these as the loss for an individual $i$ in subgroup $k$ 

\begin{align*}
		  &W_1^2=  \left( \beta_1 -  \bar{y}_1\frac{ \bar{y}_1 \beta_1 + \bar{y}_2 \beta_2 + (1 - \bar{y}_1 - \bar{y}_2) \beta_3 }{\bar{y}_1^2 + \bar{y}_2^2 + (1 - \bar{y}_1 - \bar{y}_2 )^2} \right)^2 \\
		  &W_2^2= \left( \beta_2 -  \bar{y}_2\frac{ \bar{y}_1 \beta_1 +  \bar{y}_2 \beta_2 + (1 - \bar{y}_1 - \bar{y}_2) \beta_3 }{\bar{y}_1^2 + \bar{y}_2^2 + (1 - \bar{y}_1 - \bar{y}_2 )^2} \right)^2 \\
		  &W_3^2 = \left( \beta_3 - (1 - \bar{y}_1 - \bar{y}_2)\frac{ \bar{y}_1 \beta_1 +\bar{y}_2 \beta_2 + (1 - \bar{y}_1 - \bar{y}_2) \beta_3 }{\bar{y}_1^2 + \bar{y}_2^2 + (1 - \bar{y}_1 - \bar{y}_2 )^2} \right)^2 \\
\end{align*} 


Call $\xi = \frac{ \bar{y}_1 \beta_1 + \bar{y}_2 \beta_2 + (1 - \bar{y}_1 - \bar{y}_2) \beta_3 }{\bar{y}_1^2 + \bar{y}_2^2 + (1 - \bar{y}_1 - \bar{y}_2 )^2}$

Then 

\begin{align*}
		  &W_1^2=  \left( \beta_1 -  \bar{y}_1 \xi \right)^2 = \beta_1^2 - 2 \beta_1 \bar{y}_1 \xi + \bar{y}_1^2 \xi^2 \\
		  &W_2^2= \left( \beta_2 -  \bar{y}_2 \xi \right)^2 = \beta_2^2 - 2 \beta_2 \bar{y}_2 \xi + \bar{y}_2^2 \xi^2 \\
		  &W_3^2 = \left( \beta_3 - (1 - \bar{y}_1 - \bar{y}_2) \xi \right)^2 = \beta_3^2 - 2 \beta_3 \xi(1 - \bar{y}_1 - \bar{y}_2)  + \bar{y}_3^2 \xi^2 \\
		  % & = \left( \beta_3 - (1 - \bar{y}_1 - \bar{y}_2) \xi \right)^2 = \beta_3^2 - 2 \beta_3 \xi(\bar{y}_1^2 + 2 \bar{y}_1 \bar{y}_2 - 2 \bar{y}_1 + \bar{y}_2^2 - 2 \bar{y}_2 +1)  + \bar{y}_3^2 \xi^2 \\
\end{align*} 

taking expectation over $\gamma_i$ we get

\begin{align*}
		  &W_1^2=  \Var(\gamma_1) - 2 \Var(\beta_1) \frac{\bar{y}_1^2}{\bar{y}_1^2 + \bar{y}_2^2 + (1 - \bar{y}_1 - \bar{y}_2 )^2} + \bar{y}_1^2 \xi^2 \\
		  &W_2^2=  \Var(\gamma_2) - 2 \Var(\beta_2) \frac{\bar{y}_2^2}{\bar{y}_1^2 + \bar{y}_2^2 + (1 - \bar{y}_1 - \bar{y}_2 )^2} + \bar{y}_2^2 \xi^2 \\
		  &W_3^2=  \Var(\gamma_3) - 2 \Var(\beta_3) \frac{(1 - \bar{y}_1 - \bar{y}_2)^2}{\bar{y}_1^2 + \bar{y}_2^2 + (1 - \bar{y}_1 - \bar{y}_2 )^2} + (1 - \bar{y}_1 - \bar{y}_2)^2 \xi^2 \\
\end{align*}

and start by assuming $\Var(\gamma_i) = 1$ then

\begin{align*}
	J = &p_1 W_1^2 + p_2 W_2^2 + p_3 W_3^2 \\
	J = &p_1[1 - 2 \frac{\bar{y}_1^2}{\bar{y}_1^2 + \bar{y}_2^2 + (1 - \bar{y}_1 - \bar{y}_2 )^2}+ \bar{y}_1^2 \xi^2] \\
	+ &p_2 [1 - 2 \frac{\bar{y}_2^2}{\bar{y}_1^2 + \bar{y}_2^2 + (1 - \bar{y}_1 - \bar{y}_2 )^2}+ \bar{y}_2^2 \xi^2 ] + \\
	  &(1-p_1 - p_2) [1 -2 \frac{(1-\bar{y}_1 - \bar{y}_2)^2}{\bar{y}_1^2 + \bar{y}_2^2 + (1 - \bar{y}_1 - \bar{y}_2 )^2} + (1-\bar{y}_1 - \bar{y}_2)^2 \xi^2] \\
\end{align*}

First, assume $p = p_1 = p_2 = p_3 = \frac{1}{3}$
            
and note that in expectation (assuming $Cov(\gamma_i, \gamma_j) = 0$ for $i \neq j$)
\begin{align*}
	(\bar{y}_1 \beta_1 + \bar{y}_2 \beta_2 + (1 - \bar{y}_1 - \bar{y}_2) \beta_3 )^2 &= \Var(\gamma_1) \bar{y}_1^2 + \Var(\gamma_2) \bar{y}_2^2 + \Var(\gamma_3) (1 - \bar{y}_1 - \bar{y}_2)^2 \\
																					 &=  \bar{y}_1^2 +  \bar{y}_2^2 +  (1 - \bar{y}_1 - \bar{y}_2)^2 \\
\end{align*}

In other words, in expectation
\begin{align*}
	\xi^2 = \frac{1}{\bar{y}_1^2 +  \bar{y}_2^2 +  (1 - \bar{y}_1 - \bar{y}_2)^2}
\end{align*} 

then

\begin{align*}
	J = & p [3 - 2 \frac{\bar{y}_1^2 + \bar{y}_2^2 + (1 - \bar{y}_1 - \bar{y}_2 )^2}{\bar{y}_1^2 + \bar{y}_2^2 + (1 - \bar{y}_1 - \bar{y}_2 )^2} + (\bar{y}_1^2 + \bar{y}_2^2 + (1 - \bar{y}_1 - \bar{y}_2 )^2) \xi^2] \\
	= &p[3 - 2 + 1] = \frac{2}{3} \\
\end{align*} 



% Now let $p_1 = 0.5, p_2 = 0.25, p_3 = 0.25$
Now for general $p_1, p_2, p_3$

\begin{align*}
	J = &p_1 W_1^2 + p_2 W_2^2 + p_3 W_3^2 \\
	J = &p_1[1 - \frac{\bar{y}_1^2}{\bar{y}_1^2 + \bar{y}_2^2 + (1 - \bar{y}_1 - \bar{y}_2 )^2}] \\
	+ &p_2 [1 - \frac{\bar{y}_2^2}{\bar{y}_1^2 + \bar{y}_2^2 + (1 - \bar{y}_1 - \bar{y}_2 )^2}] + \\
	  &(1-p_1 - p_2) [1 -\frac{(1-\bar{y}_1 - \bar{y}_2)^2}{\bar{y}_1^2 + \bar{y}_2^2 + (1 - \bar{y}_1 - \bar{y}_2 )^2} ] \\
	  &= 1 - \frac{p_1 \bar{y}_1^2 + p_2\bar{y}_2^2 + p_3(1 - \bar{y}_1 - \bar{y}_2 )^2}{\bar{y}_1^2 + \bar{y}_2^2 + (1 - \bar{y}_1 - \bar{y}_2 )^2} \\
	  &= \frac{(1-p_1) \bar{y}_1^2 + (1-p_2)\bar{y}_2^2 + (1-p_3)(1 - \bar{y}_1 - \bar{y}_2 )^2}{\bar{y}_1^2 + \bar{y}_2^2 + (1 - \bar{y}_1 - \bar{y}_2 )^2}
\end{align*}


\begin{align*}
	\frac{d}{dx}& \frac{ (1 - p_1) x^2 + (1 - p_2) y^2 + (1 - p_1 - p_2) (1 - x - y)^2 }{ x^2 + y^2 + (1 - x - y)^2 } = 0 \\
	&\frac{ 2 p_2 x (x (y - 1) + 2 y^2 - 2 y + 1) - 2 p_1 y^2 (2 x + y - 1) }{( x^2 + y^2 + (1 - x - y)^2 )^2} = 0\\
	\frac{d}{dy} &\frac{ (1 - p_1) x^2 + (1 - p_2) y^2 + (1 - p_1 - p_2) (1 - x - y)^2 }{ x^2 + y^2 + (1 - x - y)^2 } = 0 \\
				 &\frac{ 2 p_1 y (2 x^2 + x (y - 2) - y + 1) - 2 p_2 x^2 (x + 2 y - 1) }{( x^2 + y^2 + (1 - x - y)^2 )^2} = 0
\end{align*} 

We must solve the system of equations

\begin{align*}
	&2 p_2 x (x (y - 1) + 2 y^2 - 2 y + 1) - 2 p_1 y^2 (2 x + y - 1) = 0 \\
	&2 p_1 y (2 x^2 + x (y - 2) - y + 1) - 2 p_2 x^2 (x + 2 y - 1) = 0
\end{align*} 

we can immediately see that $x=0$ and $y=1$ are always solutions. Likewise $(x,y) = (0,0)$ is also always a solution.
We only need to investigate whether the Heissian is positive definite or not to determine which one is a minimum and which is a maximum


