
\subsection*{5. Generalization allowing for $k$ subgroups.}

again we assume $\Var(\gamma_i) = 1$ and $\Cov(\gamma_i, \gamma_j) = 0$ for $i \neq j$

we saw from before that we can write

\begin{align*}
	E J_i &= p_1 ( \alpha_1 - c_1 (\bar{y}_1 \alpha_1 + \bar{y}_2 \alpha_2 + \ldots + \bar{y}_k \alpha_k ))^2 \\
		  &+ p_2 ( \alpha_2 - c_2 (\bar{y}_1 \alpha_1 +  \bar{y}_2 \alpha_2 + \ldots + \bar{y}_k \alpha_k ))^2 \\
		  &\vdots \\
		  &+ p_k ( \alpha_k - c_k (\bar{y}_1 \alpha_1 +\bar{y}_2 \alpha_2 +  \ldots + \bar{y}_k \alpha_k ))^2 \\
\end{align*}

expanding $c_i$ 

We can describe these as the loss for an individual $i$ in subgroup $k$ 

\begin{align*}
		  &W_1^2=  \left( \alpha_1 -  \bar{y}_1\frac{ \bar{y}_1 \alpha_1 + \bar{y}_2 \alpha_2 + \ldots + \bar{y}_k \alpha_k }{\bar{y}_1^2 + \bar{y}_2^2 + \ldots + \bar{y}_k^2} \right)^2 \\
		  &W_2^2= \left( \alpha_2 -  \bar{y}_2\frac{ \bar{y}_1 \alpha_1 + \bar{y}_2 \alpha_2 + \ldots + \bar{y}_k \alpha_k }{\bar{y}_1^2 + \bar{y}_2^2 + \ldots + \bar{y}_k^2} \right)^2 \\
		  &W_3^2 = \left( \alpha_3 - \bar{y}_k\frac{ \bar{y}_1 \alpha_1 + \bar{y}_2 \alpha_2 + \ldots + \bar{y}_k \alpha_k }{\bar{y}_1^2 + \bar{y}_2^2 + \ldots + \bar{y}_k^2} \right)^2 \\
\end{align*} 

where $\bar{y}_k = (1 - \bar{x}_1 - \ldots - \bar{y}_{k-1}$


Call $\xi = \frac{ \bar{y}_1 \alpha_1 + \bar{y}_2 \alpha_2 + \ldots + \bar{y}_k \alpha_k }{\bar{y}_1^2 + \bar{y}_2^2 + \ldots + \bar{y}_k^2}$


\begin{align*}
		  &W_1^2=  \left( \alpha_1 -  \bar{y}_1 \xi \right)^2 = \alpha_1^2 - 2 \alpha_1 \bar{y}_1 \xi + \bar{y}_1^2 \xi^2 \\
		  &W_2^2= \left( \alpha_2 -  \bar{y}_2 \xi \right)^2 = \alpha_2^2 - 2 \alpha_2 \bar{y}_2 \xi + \bar{y}_2^2 \xi^2 \\
		  &W_3^2 = \left( \alpha_3 - (1 - \bar{y}_1 - \bar{y}_2) \xi \right)^2 = \alpha_3^2 - 2 \alpha_3 \xi(1 - \bar{y}_1 - \bar{y}_2)  + \bar{y}_3^2 \xi^2 \\
		  % & = \left( \alpha_3 - (1 - \bar{y}_1 - \bar{y}_2) \xi \right)^2 = \alpha_3^2 - 2 \alpha_3 \xi(\bar{y}_1^2 + 2 \bar{y}_1 \bar{y}_2 - 2 \bar{y}_1 + \bar{y}_2^2 - 2 \bar{y}_2 +1)  + \bar{y}_3^2 \xi^2 \\
\end{align*} 

taking expectation over $\gamma_i$ we get

\begin{align*}
		  &W_1^2=  \Var(\gamma_1) - 2 \Var(\gamma_1) \frac{\bar{y}_1^2}{\bar{y}_1^2 + \bar{y}_2^2 + (1 - \bar{y}_1 - \bar{y}_2 )^2} + \bar{y}_1^2 \xi^2 \\
		  &W_2^2=  \Var(\gamma_2) - 2 \Var(\gamma_2) \frac{\bar{y}_2^2}{\bar{y}_1^2 + \bar{y}_2^2 + (1 - \bar{y}_1 - \bar{y}_2 )^2} + \bar{y}_2^2 \xi^2 \\
		  &W_3^2=  \Var(\gamma_3) - 2 \Var(\gamma_3) \frac{(1 - \bar{y}_1 - \bar{y}_2)^2}{\bar{y}_1^2 + \bar{y}_2^2 + (1 - \bar{y}_1 - \bar{y}_2 )^2} + (1 - \bar{y}_1 - \bar{y}_2)^2 \xi^2 \\
\end{align*}

and start by assuming $\Var(\gamma_i) = 1$ then

\begin{align*}
	J = &p_1 W_1^2 + p_2 W_2^2 + p_3 W_3^2 \\
	J = &p_1[1 - 2 \frac{\bar{y}_1^2}{\bar{y}_1^2 + \bar{y}_2^2 + (1 - \bar{y}_1 - \bar{y}_2 )^2}+ \bar{y}_1^2 \xi^2] \\
	+ &p_2 [1 - 2 \frac{\bar{y}_2^2}{\bar{y}_1^2 + \bar{y}_2^2 + (1 - \bar{y}_1 - \bar{y}_2 )^2}+ \bar{y}_2^2 \xi^2 ] + \\
	  &(1-p_1 - p_2) [1 -2 \frac{(1-\bar{y}_1 - \bar{y}_2)^2}{\bar{y}_1^2 + \bar{y}_2^2 + (1 - \bar{y}_1 - \bar{y}_2 )^2} + (1-\bar{y}_1 - \bar{y}_2)^2 \xi^2] \\
\end{align*}

First, assume $p = p_1 = p_2 = p_3 = \frac{1}{3}$
            
and note that in expectation (assuming $Cov(\gamma_i, \gamma_j) = 0$ for $i \neq j$)
\begin{align*}
	(\bar{y}_1 \alpha_1 + \bar{y}_2 \alpha_2 + (1 - \bar{y}_1 - \bar{y}_2) \alpha_3 )^2 &= \Var(\gamma_1) \bar{y}_1^2 + \Var(\gamma_2) \bar{y}_2^2 + \Var(\gamma_3) (1 - \bar{y}_1 - \bar{y}_2)^2 \\
																					 &=  \bar{y}_1^2 +  \bar{y}_2^2 +  (1 - \bar{y}_1 - \bar{y}_2)^2 \\
\end{align*}

